ironfleet/src/Dafny/Distributed/Common/Reduction/UltimateRefinement.i.dfy
@@ -35,6 +35,16 @@ module UltimateRefinementModule {
         Entry(entry.actor, if entry.action.RealActionEvent? then ExtendedActionEvent(entry.action.e) else ExtendedActionUntrackedEvent(entry.action.u))
     }
 
+    function ConvertRealTraceToExtendedTrace(trace:RealTrace) : ExtendedTrace
+    {
+        ConvertMapToSeq(|trace|, map i | 0 <= i < |trace| :: ConvertRealEntryToExtendedEntry(trace[i]))
+    }
+
+    function ConvertEventsToExtendedTrace(events:seq<Event>, actor:Actor) : ExtendedTrace
+    {
+        ConvertMapToSeq(|events|, map i | 0 <= i < |events| :: Entry(actor, ExtendedActionEvent(events[i])))
+    }
+
     function EventSequenceToTree(events:seq<Event>, actor:Actor, pivot_index:int) : Tree
     {
         Inner(Entry(actor, ExtendedActionPerformIos(events)),
@@ -89,7 +99,8 @@ module UltimateRefinementModule {
         ensures  |pivot_indices| == |host_history.event_seqs|;
         ensures  forall i :: 0 <= i < |pivot_indices| ==> IsValidPivotIndexForEventSequence(pivot_indices[i], actor, host_history.event_seqs[i]);
         ensures  forall i :: 0 <= i < |pivot_indices| ==> var tree := EventSequenceToTree(host_history.event_seqs[i], actor, pivot_indices[i]);
-                       EntriesReducibleToEntry(GetRootEntries(tree.children), GetRootEntry(tree)) && LeftMoversAlwaysEnabled(tree);
+                    EntriesReducibleToEntry(GetRootEntries(tree.children), GetRootEntry(tree))
+                 && LeftMoversAlwaysEnabled(tree);
     {
         var pos := 0;
         pivot_indices := [];
@@ -98,7 +109,8 @@ module UltimateRefinementModule {
             invariant |pivot_indices| == pos;
             invariant forall i :: 0 <= i < pos ==> IsValidPivotIndexForEventSequence(pivot_indices[i], actor, host_history.event_seqs[i]);
             invariant forall i :: 0 <= i < pos ==> var tree := EventSequenceToTree(host_history.event_seqs[i], actor, pivot_indices[i]);
-                       EntriesReducibleToEntry(GetRootEntries(tree.children), GetRootEntry(tree)) && LeftMoversAlwaysEnabled(tree);
+                            EntriesReducibleToEntry(GetRootEntries(tree.children), GetRootEntry(tree))
+                         && LeftMoversAlwaysEnabled(tree);
         {
             var hb := host_history.states[..pos+1];
             var ios_seq := host_history.event_seqs[..pos];
@@ -177,8 +189,10 @@ module UltimateRefinementModule {
         requires forall actor :: actor in completed_actors <==> actor in partial_plan;
         requires forall actor :: actor in completed_actors ==> IsValidActorReductionPlan(config, partial_plan[actor], actor);
         requires forall actor :: actor in completed_actors ==> TreesOnlyForActor(partial_plan[actor].trees, actor);
+        requires forall actor :: actor in completed_actors ==> GetLeafEntriesForest(partial_plan[actor].trees) == ConvertEventsToExtendedTrace(ConcatenateEventSequences(host_histories[actor].event_seqs), actor);
         ensures  forall actor :: actor in TrackedActorsInConfig(config) <==> actor in plan;
         ensures  IsValidReductionPlan(config, plan);
+        ensures  forall actor :: actor in TrackedActorsInConfig(config) ==> GetLeafEntriesForest(plan[actor].trees) == ConvertEventsToExtendedTrace(ConcatenateEventSequences(host_histories[actor].event_seqs), actor);
         decreases |TrackedActorsInConfig(config) - completed_actors|;
     {
         if completed_actors == TrackedActorsInConfig(config) {
@@ -190,6 +204,8 @@ module UltimateRefinementModule {
         var host_history := host_histories[actor];
         var pivot_indices := ComputePivotIndicesForHostHistory(config, host_history, actor);
         var actor_reduction_plan := HostHistoryToActorReductionPlan(host_history, actor, pivot_indices);
+
+        lemma_GetLeafEntriesForestForTrees(actor_reduction_plan.trees, host_history.event_seqs, actor, pivot_indices);
 
         forall idx {:trigger actor_reduction_plan.trees[idx]} | 0 <= idx < |actor_reduction_plan.trees|
             ensures TreeValid(actor_reduction_plan.trees[idx]);
@@ -209,7 +225,138 @@ module UltimateRefinementModule {
         plan := ComputeReductionPlanFromHostHistories(config, host_histories, updated_plan, completed_actors + {actor});
     }
 
-    lemma RefinementProofAlt(
+    lemma lemma_GetLeafEntriesForTree(
+        tree:Tree,
+        event_seq:seq<Event>,
+        actor:Actor,
+        pivot_index:int
+        )
+        requires tree == EventSequenceToTree(event_seq, actor, pivot_index);
+        ensures  GetLeafEntries(tree) == ConvertEventsToExtendedTrace(event_seq, actor);
+        decreases |event_seq|;
+    {
+        if |event_seq| == 0 {
+            return;
+        }
+
+        var event_seq' := event_seq[1..];
+        var tree' := EventSequenceToTree(event_seq', actor, pivot_index);
+        assert tree'.children == tree.children[1..];
+        lemma_GetLeafEntriesForTree(tree', event_seq', actor, pivot_index);
+
+        calc {
+            GetLeafEntries(tree);
+            GetLeafEntriesForest(tree.children);
+            GetLeafEntries(tree.children[0]) + GetLeafEntriesForest(tree.children[1..]);
+            GetLeafEntries(tree.children[0]) + GetLeafEntriesForest(tree'.children);
+            GetLeafEntries(tree.children[0]) + GetLeafEntries(tree');
+            GetLeafEntries(tree.children[0]) + ConvertEventsToExtendedTrace(event_seq', actor);
+            [Entry(actor, ExtendedActionEvent(event_seq[0]))] + ConvertEventsToExtendedTrace(event_seq', actor);
+            ConvertEventsToExtendedTrace(event_seq, actor);
+        }
+    }
+
+    lemma lemma_GetLeafEntriesForestForTrees(
+        trees:seq<Tree>,
+        event_seqs:seq<seq<Event>>,
+        actor:Actor,
+        pivot_indices:seq<int>
+        )
+        requires |trees| == |event_seqs| == |pivot_indices|;
+        requires forall i :: 0 <= i < |trees| ==> trees[i] == EventSequenceToTree(event_seqs[i], actor, pivot_indices[i]);
+        ensures GetLeafEntriesForest(trees) == ConvertEventsToExtendedTrace(ConcatenateEventSequences(event_seqs), actor);
+    {
+        if |trees| == 0 {
+            return;
+        }
+
+        var trees' := trees[1..];
+        var event_seqs' := event_seqs[1..];
+        var pivot_indices' := pivot_indices[1..];
+        lemma_GetLeafEntriesForestForTrees(trees', event_seqs', actor, pivot_indices');
+
+        calc {
+            GetLeafEntriesForest(trees);
+            GetLeafEntries(trees[0]) + GetLeafEntriesForest(trees');
+            GetLeafEntries(trees[0]) + ConvertEventsToExtendedTrace(ConcatenateEventSequences(event_seqs'), actor);
+            { lemma_GetLeafEntriesForTree(trees[0], event_seqs[0], actor, pivot_indices[0]); }
+            ConvertEventsToExtendedTrace(event_seqs[0], actor) + ConvertEventsToExtendedTrace(ConcatenateEventSequences(event_seqs'), actor);
+            ConvertEventsToExtendedTrace(event_seqs[0] + ConcatenateEventSequences(event_seqs'), actor);
+            ConvertEventsToExtendedTrace(ConcatenateEventSequences(event_seqs), actor);
+        }
+    }
+
+    lemma lemma_RestrictTraceToTrackedEventsPreservedAcrossConversion(
+        rtrace:RealTrace,
+        etrace:ExtendedTrace,
+        rtrace_tracked:RealTrace,
+        etrace_tracked:ExtendedTrace
+        )
+        requires etrace == ConvertRealTraceToExtendedTrace(rtrace);
+        requires rtrace_tracked == RestrictRealTraceToTrackedEvents(rtrace);
+        requires etrace_tracked == RestrictTraceToTrackedActions(etrace);
+        ensures  etrace_tracked == ConvertRealTraceToExtendedTrace(rtrace_tracked);
+    {
+        if |rtrace| == 0 {
+            return;
+        }
+
+        var rtrace' := rtrace[1..];
+        var etrace' := etrace[1..];
+        var rtrace_tracked' := RestrictRealTraceToTrackedEvents(rtrace');
+        var etrace_tracked' := RestrictTraceToTrackedActions(etrace');
+        lemma_RestrictTraceToTrackedEventsPreservedAcrossConversion(rtrace', etrace', rtrace_tracked', etrace_tracked');
+    }
+
+    lemma lemma_RestrictTraceToActorPreservedAcrossConversion(
+        actor:Actor,
+        rtrace:RealTrace,
+        etrace:ExtendedTrace,
+        rtrace_restricted:RealTrace,
+        etrace_restricted:ExtendedTrace
+        )
+        requires etrace == ConvertRealTraceToExtendedTrace(rtrace);
+        requires rtrace_restricted == RestrictTraceToActor(rtrace, actor);
+        requires etrace_restricted == RestrictTraceToActor(etrace, actor);
+        ensures  etrace_restricted == ConvertRealTraceToExtendedTrace(rtrace_restricted);
+    {
+        if |rtrace| == 0 {
+            return;
+        }
+
+        var rtrace' := rtrace[1..];
+        var etrace' := etrace[1..];
+        var rtrace_restricted' := RestrictTraceToActor(rtrace', actor);
+        var etrace_restricted' := RestrictTraceToActor(etrace', actor);
+        lemma_RestrictTraceToActorPreservedAcrossConversion(actor, rtrace', etrace', rtrace_restricted', etrace_restricted');
+    }
+
+    lemma lemma_ConvertRealBehaviorToExtendedBehaviorRefinementTranslation(
+        config:ConcreteConfiguration,
+        rb:seq<RealSystemState>,
+        eb:seq<ExtendedSystemState>
+        )
+        requires BehaviorRefinesSpec(eb, GetSpec(config), GetExtendedSystemSpecRefinementRelation());
+        requires |rb| == |eb|;
+        requires forall i :: 0 <= i < |rb| ==> eb[i].ss == rb[i];
+        ensures  BehaviorRefinesSpec(rb, GetSpec(config), GetRealSystemSpecRefinementRelation());
+    {
+        var spec := GetSpec(config);
+        var extended_relation := GetExtendedSystemSpecRefinementRelation();
+        var hb :| BehaviorRefinesBehavior(eb, hb, extended_relation) && BehaviorSatisfiesSpec(hb, spec);
+        var lh_map :| BehaviorRefinesBehaviorUsingRefinementMap(eb, hb, extended_relation, lh_map);
+
+        var real_relation := GetRealSystemSpecRefinementRelation();
+        forall i, j {:trigger RefinementPair(rb[i], hb[j]) in real_relation} | 0 <= i < |rb| && lh_map[i].first <= j <= lh_map[i].last
+            ensures RefinementPair(rb[i], hb[j]) in real_relation;
+        {
+            assert RefinementPair(eb[i], hb[j]) in extended_relation;
+        }
+        assert BehaviorRefinesBehaviorUsingRefinementMap(rb, hb, real_relation, lh_map);
+        assert BehaviorRefinesBehavior(rb, hb, real_relation);
+    }
+
+    lemma lemma_RefinementProofByReduction(
         config:ConcreteConfiguration,
         trace:RealTrace,
         host_histories:map<Actor, HostHistory>,
@@ -223,11 +370,11 @@ module UltimateRefinementModule {
                      && !actor.NoActor?
                      && actor in host_histories
                      && IsValidHostHistory(config, host_histories[actor], actor)
-                     && EventSequenceToTrace(ConcatenateEventSequences(host_histories[actor].event_seqs), actor) ==
-                        RestrictTraceToActor(trace, actor);
+                     && RestrictTraceToActor(RestrictRealTraceToTrackedEvents(trace), actor) <=
+                        EventSequenceToTrace(ConcatenateEventSequences(host_histories[actor].event_seqs), actor);
         ensures  BehaviorRefinesSpec(rb, GetSpec(config), GetRealSystemSpecRefinementRelation());
     {
-        var etrace := ConvertMapToSeq(|trace|, map i | 0 <= i < |trace| :: ConvertRealEntryToExtendedEntry(trace[i]));
+        var etrace := ConvertRealTraceToExtendedTrace(trace);
         var eb := ConvertMapToSeq(|rb|, map i | 0 <= i < |rb| :: ExtendedSystemState(map [], rb[i]));
         var plan := ComputeReductionPlanFromHostHistories(config, host_histories, map [], {});
 
@@ -237,10 +384,34 @@ module UltimateRefinementModule {
             assert SystemNextEntry(rb[i], rb[i+1], trace[i]);
         }
 
-        assume forall actor :: actor in TrackedActorsInConfig(config) ==>
-                     RestrictTraceToActor(RestrictTraceToTrackedActions(etrace), actor) <= GetLeafEntriesForest(plan[actor].trees);
+        forall actor | actor in TrackedActorsInConfig(config)
+            ensures RestrictTraceToActor(RestrictTraceToTrackedActions(etrace), actor) <= GetLeafEntriesForest(plan[actor].trees);
+        {
+            var real_trace_tracked := RestrictRealTraceToTrackedEvents(trace);
+            var real_actor_trace_tracked := RestrictTraceToActor(real_trace_tracked, actor);
+            var concatenated_histories := ConcatenateEventSequences(host_histories[actor].event_seqs);
+            var concatenated_histories_trace := EventSequenceToTrace(concatenated_histories, actor);
+            var leaf_entries_forest := GetLeafEntriesForest(plan[actor].trees);
+            var etrace_tracked := RestrictTraceToTrackedActions(etrace);
+            var etrace_actor_tracked := RestrictTraceToActor(etrace_tracked, actor);
+
+            calc {
+                etrace_actor_tracked;
+                {
+                    lemma_RestrictTraceToTrackedEventsPreservedAcrossConversion(trace, etrace, real_trace_tracked, etrace_tracked);
+                    lemma_RestrictTraceToActorPreservedAcrossConversion(actor, real_trace_tracked, etrace_tracked, real_actor_trace_tracked,
+                                                                        etrace_actor_tracked);
+                }
+                ConvertRealTraceToExtendedTrace(real_actor_trace_tracked);
+                <= ConvertRealTraceToExtendedTrace(concatenated_histories_trace);
+                ConvertRealTraceToExtendedTrace(EventSequenceToTrace(concatenated_histories, actor));
+                ConvertEventsToExtendedTrace(concatenated_histories, actor);
+                leaf_entries_forest;
+            }
+        }
+
         lemma_UltimateRefinement(config, etrace, eb, plan);
-        assume false;
+        lemma_ConvertRealBehaviorToExtendedBehaviorRefinementTranslation(config, rb, eb);
     }
 
 }
